examples/opaque/server_proofs.v
@@ -24,7 +24,10 @@ Notation iProp := (iProp Σ).
 Definition opaque_file (file : val) : iProp :=
   ∃ k_s p_s P_s P_u envelope,
     ⌜file = Spec.of_list [k_s; p_s; P_s; P_u; envelope]⌝
-    ∗ minted k_s ∗ □(∀ t' : term, dh_pred k_s t' ↔ ▷ □ True) ∗ minted p_s ∗ public P_s ∗ public P_u ∗ public envelope.
+    ∗ minted k_s ∗
+    □(∀ t' : term, dh_pred_base k_s t' ↔ ▷ □ True) ∗
+    □(∀ t' : term, dh_pred_base (TInv k_s) t' ↔ ▷ False) ∗
+    minted p_s ∗ public P_s ∗ public P_u ∗ public envelope.
 
 Definition opaque_db (db : gmap term val) : iProp :=
 [∗ map] (k : term) ↦ (file : val) ∈ db,
@@ -60,7 +63,7 @@ Proof.
   iIntros "%ϕ [#cryptis [#Hmintedpw [#Hprivpw [#Hhashpred [#Hsencpred #Henc]]]]] post".
   wp_lam.
   wp_apply (wp_mk_nonce (fun _ => False)%I (fun _ => True)%I) => //.
-  iIntros "%k_s %Hnoncek_s #Hmintedk_s #Hprivatek_s #Heqk_s Htokenk_s".
+  iIntros "%k_s %Hnoncek_s #Hmintedk_s #Hprivatek_s #Heqk_s #Heqk_sV Htokenk_s".
   wp_pures.
   wp_lam.
   wp_pures.
@@ -71,10 +74,10 @@ Proof.
   wp_apply wp_derive_senc_key.
   wp_pures.
   wp_apply (wp_mk_nonce (fun _ => False)%I (fun _ => True)%I) => //.
-  iIntros "%p_s %Hnoncep_s #Hmintedp_s #Hprivatep_s #Heqp_s Htokenp_s".
+  iIntros "%p_s %Hnoncep_s #Hmintedp_s #Hprivatep_s #Heqp_s #Heqp_sV Htokenp_s".
   wp_pures.
   wp_apply (wp_mk_nonce (fun _ => False)%I (fun _ => True)%I) => //.
-  iIntros "%p_u %Hnoncep_u #Hmintedp_u #Hprivatep_u #Heqp_u Htokenp_u".
+  iIntros "%p_u %Hnoncep_u #Hmintedp_u #Hprivatep_u #Heqp_u #Heqp_uV Htokenp_u".
   wp_pures.
   wp_apply wp_texp. wp_pures.
   wp_apply wp_texp.
@@ -90,8 +93,10 @@ Proof.
   1, 2: iApply public_TExp_iff; auto.
   1, 2: iRight; do !iSplit => //.
   1, 4: by iApply minted_TInt.
+  iApply dh_pred_intro1.
   by iApply "Heqp_s"; auto.
   1, 3: by rewrite public_TInt; auto.
+  iApply dh_pred_intro1.
   by iApply "Heqp_u"; auto.
   iApply (public_sencIS _ (opN.@"AuthEnc") Φ _) => //.
   rewrite minted_senc minted_THash minted_tag.
@@ -142,7 +147,7 @@ Proof.
   2: by iApply "Hhl".
   iDestruct ("Hmapcontents" $! uid file with "[//]") as
   "[_ (%k_s & %p_s & %P_s & %P_u & %envelope &
-        %e & Hmk_s & Hdhpredk_s & Hmp_s & HpP_s & HpP_u & Hpenvelope)]".
+        %e & Hmk_s & Hdhpredk_s & Hmp_s & Hmp_sV & HpP_s & HpP_u & Hpenvelope)]".
   rewrite !subst_list_match /= e.
   wp_apply wp_list_of_term.
   rewrite Spec.of_listK.
@@ -152,7 +157,7 @@ Proof.
   inversion e'. subst. clear e'.
   2: by intro contra.
   wp_apply (wp_mk_nonce (fun _ => False)%I (fun _ => True)%I) => //.
-  iIntros "%x_s %Hnoncex_s #Hmintedx_s #Hprivatex_s #Hdhx_s Htokenx_s".
+  iIntros "%x_s %Hnoncex_s #Hmintedx_s #Hprivatex_s #Hdhx_s #Hdhx_sV Htokenx_s".
   wp_pures.
   wp_apply wp_texp. wp_pures.
   wp_apply wp_texp. wp_pures.
@@ -177,6 +182,7 @@ Proof.
   iRight.
   do !iSplit => //.
   by iApply minted_TInt.
+  iApply dh_pred_intro1.
   by iApply "Hdhx_s"; auto.
   by rewrite public_TInt; auto.
   iApply public_THashIS => //.
